language/move-prover/src/spec_translator.rs
@@ -3,7 +3,7 @@
 
 //! This module translates specification conditions to Boogie code.
 
-use std::{cell::RefCell, collections::BTreeMap};
+use std::{cell::RefCell, rc::Rc};
 
 use spec_lang::{
     env::{FieldId, Loc, ModuleEnv, ModuleId, NodeId, SpecFunId, StructEnv, StructId},
@@ -45,13 +45,13 @@ pub struct SpecTranslator<'env> {
     supports_native_old: bool,
     /// Whether we are currently in the context of translating an `old(...)` expression.
     in_old: RefCell<bool>,
+    /// Whether we are currently translating an ensures specification.
+    in_ensures: RefCell<bool>,
     /// The current target for invariant fields, a pair of strings for current and old value.
     invariant_target: RefCell<(String, String)>,
     /// Counter for generating fresh variables.  It's a RefCell so we can increment it without
     /// making a ton of &self arguments mutable.
     fresh_var_count: RefCell<u64>,
-    /// Local variable name to local index in bytecode
-    name_to_idx_map: BTreeMap<Symbol, usize>,
     // If we are translating in the context of a type instantiation, the type arguments.
     type_args_opt: Option<Vec<Type>>,
 }
@@ -89,9 +89,9 @@ impl<'env> SpecTranslator<'env> {
             writer,
             supports_native_old,
             in_old: RefCell::new(false),
+            in_ensures: RefCell::new(false),
             invariant_target: RefCell::new(("".to_string(), "".to_string())),
             fresh_var_count: RefCell::new(0),
-            name_to_idx_map: BTreeMap::new(),
             type_args_opt: None,
         }
     }
@@ -107,11 +107,9 @@ impl<'env> SpecTranslator<'env> {
             writer,
             supports_native_old,
             in_old: RefCell::new(false),
+            in_ensures: RefCell::new(false),
             invariant_target: RefCell::new(("".to_string(), "".to_string())),
             fresh_var_count: RefCell::new(0),
-            name_to_idx_map: (0..func_target.get_local_count())
-                .map(|idx| (func_target.get_local_name(idx), idx))
-                .collect(),
             type_args_opt: None,
         }
     }
@@ -368,12 +366,14 @@ impl<'env> SpecTranslator<'env> {
         // Generate ensures
         let ensures = spec.filter_kind(ConditionKind::Ensures).collect_vec();
         if !ensures.is_empty() {
+            *self.in_ensures.borrow_mut() = true;
             self.translate_seq(ensures.iter(), "\n", |cond| {
                 self.writer.set_location(&cond.loc);
                 emit!(self.writer, "ensures !$abort_flag ==> (b#Boolean(");
                 self.translate_exp(&cond.exp);
                 emit!(self.writer, "));")
             });
+            *self.in_ensures.borrow_mut() = false;
             emitln!(self.writer);
         }
     }
@@ -495,20 +495,13 @@ impl<'env> SpecTranslator<'env> {
     }
 
     /// Determines whether a before-update invariant is generated for this struct.
-    ///
-    /// We currently support two models for dealing with global spec var updates.
-    /// If the specification has explicitly provided update invariants for spec vars, we use those.
-    /// If not, we use the unpack invariants before the update, and the pack invariants
-    /// after. This function is only true for the later case.
     pub fn has_before_update_invariant(struct_env: &StructEnv<'_>) -> bool {
-        let spec = struct_env.get_spec();
-        let no_explict_update = !spec.any(|c| matches!(c.kind, ConditionKind::VarUpdate(..)));
-        let has_pack = spec.any(|c| matches!(c.kind, ConditionKind::VarPack(..)));
-        no_explict_update && has_pack
-            // If any of the fields has it, it inherits to the struct.
-            || struct_env.get_fields().any(|fe| {
-                Self::has_before_update_invariant_ty(struct_env.module_env.env, &fe.get_type())
-            })
+        use ConditionKind::*;
+        struct_env.get_spec().any(|c| matches!(c.kind, VarUpdate(..)|VarUnpack(..)|Invariant))
+                // If any of the fields has it, it inherits to the struct.
+                || struct_env.get_fields().any(|fe| {
+                    Self::has_before_update_invariant_ty(struct_env.module_env.env, &fe.get_type())
+                })
     }
 
     /// Determines whether a before-update invariant is generated for this type.
@@ -566,6 +559,15 @@ impl<'env> SpecTranslator<'env> {
             }
         }
 
+        // Emit data invariants for this struct.
+        let spec = struct_env.get_spec();
+        self.emit_invariants_assume_or_assert(
+            "$before",
+            "",
+            true,
+            spec.filter_kind(ConditionKind::Invariant),
+        );
+
         // Emit call to spec var updates via unpack invariants.
         self.emit_spec_var_updates(
             "$before",
@@ -611,7 +613,7 @@ impl<'env> SpecTranslator<'env> {
             boogie_struct_name(struct_env),
             Self::translate_type_parameters(struct_env)
                 .into_iter()
-                .chain(vec!["$before: Value, $after: Value".to_string()])
+                .chain(vec!["$after: Value".to_string()])
                 .join(", "),
         );
         self.writer.indent();
@@ -626,13 +628,7 @@ impl<'env> SpecTranslator<'env> {
                     let args = ty_args
                         .iter()
                         .map(|ty| self.translate_type(ty))
-                        .chain(
-                            vec![format!(
-                                "$SelectField($before, {}), $SelectField($after, {})",
-                                field_name, field_name
-                            )]
-                            .into_iter(),
-                        )
+                        .chain(vec![format!("$SelectField($after, {})", field_name)].into_iter())
                         .join(", ");
                     emitln!(
                         self.writer,
@@ -860,17 +856,20 @@ impl<'env> SpecTranslator<'env> {
 
     fn translate_local_var(&self, node_id: NodeId, name: Symbol) {
         let mut ty = &self.module_env().get_node_type(node_id);
+        let mut var_name = self.module_env().symbol_pool().string(name);
         // overwrite ty if func_target provides a binding for name
         if let SpecEnv::Function(func_target) = self.spec_env {
             if let Some(local_index) = func_target.get_local_index(name) {
                 ty = func_target.get_local_type(*local_index);
+                if *self.in_ensures.borrow() && !*self.in_old.borrow() {
+                    if let Some(return_index) = func_target.get_return_index(*local_index) {
+                        var_name = Rc::new(format!("$ret{}", return_index));
+                    }
+                }
             }
         };
         self.auto_dref(ty, || {
-            emit!(
-                self.writer,
-                self.module_env().symbol_pool().string(name).as_ref()
-            );
+            emit!(self.writer, var_name.as_ref());
         });
     }
 
@@ -880,7 +879,7 @@ impl<'env> SpecTranslator<'env> {
     {
         if ty.is_reference() {
             // Automatically dereference
-            emit!(self.writer, "$Dereference($m, ");
+            emit!(self.writer, "$Dereference(");
         }
         f();
         if ty.is_reference() {
@@ -917,11 +916,7 @@ impl<'env> SpecTranslator<'env> {
                 self.translate_select(*module_id, *struct_id, *field_id, args)
             }
             Operation::Local(sym) => {
-                emit!(
-                    self.writer,
-                    "$GetLocal($m, $frame + {})",
-                    self.name_to_idx_map[sym],
-                );
+                self.translate_local_var(node_id, *sym);
             }
             Operation::Result(pos) => {
                 self.auto_dref(self.function_target().get_return_type(*pos), || {
@@ -1150,7 +1145,9 @@ impl<'env> SpecTranslator<'env> {
 
     fn translate_old(&self, args: &[Exp]) {
         if self.supports_native_old {
+            *self.in_old.borrow_mut() = true;
             self.translate_primitive_call("old", args);
+            *self.in_old.borrow_mut() = false;
         } else {
             *self.in_old.borrow_mut() = true;
             self.translate_exp(&args[0]);
