language/move-prover/stackless-bytecode-generator/src/packref_analysis.rs
@@ -2,19 +2,138 @@
 // SPDX-License-Identifier: Apache-2.0
 
 use crate::{
-    borrow_analysis::{BorrowAnnotation, BorrowInfo},
+    borrow_analysis::BorrowAnnotation,
+    dataflow_analysis::{
+        AbstractDomain, DataflowAnalysis, JoinResult, StateMap, TransferFunctions,
+    },
     function_target::{FunctionTarget, FunctionTargetData},
     function_target_pipeline::{FunctionTargetProcessor, FunctionTargetsHolder},
     stackless_bytecode::{
-        AssignKind, AttrId, BorrowNode,
+        AssignKind, AttrId,
         Bytecode::{self, *},
         Operation, TempIndex,
     },
+    stackless_control_flow_graph::{BlockId, StacklessControlFlowGraph},
 };
 use itertools::Itertools;
 use spec_lang::env::FunctionEnv;
 use std::collections::{BTreeMap, BTreeSet};
 use vm::file_format::CodeOffset;
+
+/// Copy analysis
+#[derive(Debug, Clone, PartialEq)]
+struct CopyState {
+    copies: BTreeSet<TempIndex>,
+}
+
+impl CopyState {}
+
+struct CopyAnalysis<'a> {
+    func_target: &'a FunctionTarget<'a>,
+    borrow_annotation: &'a BorrowAnnotation,
+}
+
+impl<'a> CopyAnalysis<'a> {
+    fn new(func_target: &'a FunctionTarget<'a>, borrow_annotation: &'a BorrowAnnotation) -> Self {
+        Self {
+            func_target,
+            borrow_annotation,
+        }
+    }
+
+    fn analyze(
+        &mut self,
+        copies: BTreeSet<TempIndex>,
+        instrs: &[Bytecode],
+    ) -> BTreeMap<CodeOffset, CopyState> {
+        let cfg = StacklessControlFlowGraph::new_forward(instrs);
+        let initial_state = CopyState { copies };
+        let state_map = self.analyze_function(initial_state, instrs, &cfg);
+        self.post_process(&cfg, instrs, state_map)
+    }
+
+    fn post_process(
+        &mut self,
+        cfg: &StacklessControlFlowGraph,
+        instrs: &[Bytecode],
+        state_map: StateMap<CopyState, ()>,
+    ) -> BTreeMap<CodeOffset, CopyState> {
+        let mut result = BTreeMap::new();
+        for (block_id, block_state) in state_map {
+            let mut state = block_state.pre;
+            for offset in cfg.instr_indexes(block_id) {
+                let instr = &instrs[offset as usize];
+                result.insert(offset, state.clone());
+                state = self.execute(state, instr, offset).unwrap();
+            }
+        }
+        result
+    }
+
+    fn execute(
+        &mut self,
+        pre: CopyState,
+        instr: &Bytecode,
+        code_offset: CodeOffset,
+    ) -> Result<CopyState, ()> {
+        use Bytecode::*;
+        let mut post = pre;
+        match instr {
+            Assign(_, dst, _, AssignKind::Copy) => {
+                if self.func_target.get_local_type(*dst).is_reference() {
+                    post.copies.insert(*dst);
+                }
+            }
+            Assign(_, dst, src, AssignKind::Move) | Assign(_, dst, src, AssignKind::Store) => {
+                if post.copies.remove(src) {
+                    post.copies.insert(*dst);
+                }
+            }
+            _ => {}
+        }
+        let after_refs = &self
+            .borrow_annotation
+            .get_borrow_info_at(code_offset)
+            .unwrap()
+            .after
+            .all_refs();
+        post.copies = post.copies.intersection(after_refs).cloned().collect();
+        Ok(post)
+    }
+}
+
+impl<'a> TransferFunctions for CopyAnalysis<'a> {
+    type State = CopyState;
+    type AnalysisError = ();
+
+    fn execute_block(
+        &mut self,
+        block_id: BlockId,
+        pre_state: Self::State,
+        instrs: &[Bytecode],
+        cfg: &StacklessControlFlowGraph,
+    ) -> Result<Self::State, Self::AnalysisError> {
+        let mut state = pre_state;
+        for offset in cfg.instr_indexes(block_id) {
+            let instr = &instrs[offset as usize];
+            state = self.execute(state, instr, offset)?;
+        }
+        Ok(state)
+    }
+}
+
+impl<'a> DataflowAnalysis for CopyAnalysis<'a> {}
+
+impl AbstractDomain for CopyState {
+    fn join(&mut self, other: &Self) -> JoinResult {
+        if self.copies == other.copies {
+            JoinResult::Unchanged
+        } else {
+            JoinResult::Error
+        }
+    }
+}
+/// Copy Analysis ends
 
 pub struct PackrefAnalysisProcessor {}
 
@@ -31,8 +150,30 @@ impl FunctionTargetProcessor for PackrefAnalysisProcessor {
         func_env: &FunctionEnv<'_>,
         mut data: FunctionTargetData,
     ) -> FunctionTargetData {
+        if func_env.is_native() {
+            return data;
+        }
         let func_target = FunctionTarget::new(func_env, &data);
-        let mut pack_analysis = PackrefAnalysis::new(&func_target, &data.code);
+        let borrow_annotation = func_target
+            .get_annotations()
+            .get::<BorrowAnnotation>()
+            .expect("borrow annotation");
+        let copy_annotation = CopyAnalysis::new(&func_target, borrow_annotation).analyze(
+            if func_target.call_ends_lifetime() {
+                BTreeSet::new()
+            } else {
+                (0..func_target.get_parameter_count())
+                    .filter(|idx| func_target.get_local_type(*idx).is_reference())
+                    .collect()
+            },
+            &data.code,
+        );
+        let mut pack_analysis = PackrefAnalysis::new(
+            &func_target,
+            borrow_annotation,
+            &copy_annotation,
+            &data.code,
+        );
         let mut new_code = BTreeMap::new();
         for (code_offset, bytecode) in data.code.iter().enumerate() {
             new_code.insert(
@@ -71,19 +212,21 @@ impl PackrefAnnotation {
 pub struct PackrefAnalysis<'a> {
     func_target: &'a FunctionTarget<'a>,
     borrow_annotation: &'a BorrowAnnotation,
+    copy_annotation: &'a BTreeMap<CodeOffset, CopyState>,
     next_attr_id: usize,
 }
 
 impl<'a> PackrefAnalysis<'a> {
-    fn new(func_target: &'a FunctionTarget<'a>, code: &[Bytecode]) -> Self {
-        let borrow_annotation = func_target
-            .get_annotations()
-            .get::<BorrowAnnotation>()
-            .expect("borrow annotation");
-
+    fn new(
+        func_target: &'a FunctionTarget<'a>,
+        borrow_annotation: &'a BorrowAnnotation,
+        copy_annotation: &'a BTreeMap<CodeOffset, CopyState>,
+        code: &[Bytecode],
+    ) -> Self {
         Self {
             func_target,
             borrow_annotation,
+            copy_annotation,
             next_attr_id: code.len(),
         }
     }
@@ -93,40 +236,38 @@ impl<'a> PackrefAnalysis<'a> {
         code_offset: CodeOffset,
         bytecode: &Bytecode,
     ) -> PackrefInstrumentation {
-        let borrow_annotation_at = self
-            .borrow_annotation
-            .get_borrow_info_at(code_offset)
-            .unwrap();
-        let (before, mut after) = self.public_function_instrumentation(code_offset, &bytecode);
+        let (before, mut after) = self.public_function_instrumentation(code_offset, bytecode);
         match bytecode {
-            SpecBlock(..)
-            | Assign(_, _, _, AssignKind::Move)
-            | Assign(_, _, _, AssignKind::Store)
-            | Ret(..)
-            | Load(..)
-            | Branch(..)
-            | Jump(..)
-            | Label(..)
-            | Abort(..)
-            | Nop(..) => {}
+            SpecBlock(..) | Assign(..) | Ret(..) | Load(..) | Branch(..) | Jump(..) | Label(..)
+            | Abort(..) | Nop(..) => {}
             _ => {
-                after.append(&mut self.ref_create_destroy_instrumentation(
-                    bytecode,
-                    &borrow_annotation_at.before,
-                    &borrow_annotation_at.after,
-                ));
+                after.append(&mut self.ref_create_destroy_instrumentation(code_offset, bytecode));
             }
         };
         PackrefInstrumentation { before, after }
     }
 
-    fn call_ends_lifetime(&self) -> bool {
-        self.func_target.is_public()
-            && self
-                .func_target
-                .get_return_types()
-                .iter()
-                .all(|ty| !ty.is_reference())
+    fn entry_exit_instrumentation(
+        &mut self,
+        code_offset: CodeOffset,
+        at_entry: bool,
+        bytecodes: &mut Vec<Bytecode>,
+    ) {
+        if self.func_target.call_ends_lifetime() {
+            let borrow_annotation_at = self
+                .borrow_annotation
+                .get_borrow_info_at(code_offset)
+                .unwrap();
+            for idx in 0..self.func_target.get_parameter_count() {
+                if borrow_annotation_at.before.live_refs.contains(&idx) {
+                    bytecodes.push(if at_entry {
+                        Bytecode::UnpackRef(self.new_attr_id(), idx)
+                    } else {
+                        Bytecode::PackRef(self.new_attr_id(), idx)
+                    });
+                }
+            }
+        }
     }
 
     fn public_function_instrumentation(
@@ -136,12 +277,8 @@ impl<'a> PackrefAnalysis<'a> {
     ) -> (Vec<Bytecode>, Vec<Bytecode>) {
         let mut before = vec![];
         let mut after = vec![];
-        if self.call_ends_lifetime() && code_offset == 0 {
-            for idx in 0..self.func_target.get_parameter_count() {
-                if self.func_target.get_local_type(idx).is_reference() {
-                    before.push(Bytecode::UnpackRef(self.new_attr_id(), idx));
-                }
-            }
+        if code_offset == 0 {
+            self.entry_exit_instrumentation(code_offset, true, &mut before);
         }
         match &bytecode {
             Call(_, dests, Operation::Function(mid, fid, _), srcs) => {
@@ -170,13 +307,7 @@ impl<'a> PackrefAnalysis<'a> {
                 }
             }
             Ret(..) => {
-                if self.call_ends_lifetime() {
-                    for idx in 0..self.func_target.get_parameter_count() {
-                        if self.func_target.get_local_type(idx).is_reference() {
-                            before.push(Bytecode::PackRef(self.new_attr_id(), idx));
-                        }
-                    }
-                }
+                self.entry_exit_instrumentation(code_offset, false, &mut before);
             }
             _ => {}
         };
@@ -191,10 +322,14 @@ impl<'a> PackrefAnalysis<'a> {
 
     fn ref_create_destroy_instrumentation(
         &mut self,
+        code_offset: CodeOffset,
         bytecode: &Bytecode,
-        before: &BorrowInfo,
-        after: &BorrowInfo,
     ) -> Vec<Bytecode> {
+        let borrow_annotation_at = self
+            .borrow_annotation
+            .get_borrow_info_at(code_offset)
+            .unwrap();
+        let copy_annotation_at = &self.copy_annotation[&code_offset];
         let mut instrumented_bytecodes = vec![];
         match bytecode {
             Call(_, dests, op, _) => {
@@ -205,34 +340,15 @@ impl<'a> PackrefAnalysis<'a> {
                             .push(Bytecode::UnpackRef(self.new_attr_id(), dests[0]));
                     }
                     _ => {
-                        let filter_fn = |node: &BorrowNode| {
-                            if let BorrowNode::Reference(idx) = node {
-                                Some(*idx)
-                            } else {
-                                None
-                            }
-                        };
-                        let before_borrowed_by =
-                            before.borrowed_by.keys().filter_map(filter_fn).collect();
-                        let before_refs: BTreeSet<&TempIndex> =
-                            before.live_refs.union(&before_borrowed_by).collect();
-                        let after_borrowed_by =
-                            after.borrowed_by.keys().filter_map(filter_fn).collect();
-                        let after_refs: BTreeSet<&TempIndex> =
-                            after.live_refs.union(&after_borrowed_by).collect();
+                        let before_refs = borrow_annotation_at.before.all_refs();
+                        let after_refs = borrow_annotation_at.after.all_refs();
                         for idx in before_refs.difference(&after_refs) {
-                            instrumented_bytecodes
-                                .push(Bytecode::PackRef(self.new_attr_id(), **idx));
+                            if !copy_annotation_at.copies.contains(idx) {
+                                instrumented_bytecodes
+                                    .push(Bytecode::PackRef(self.new_attr_id(), *idx));
+                            }
                         }
                     }
-                }
-            }
-            Assign(_, dest, _, AssignKind::Copy) => {
-                if after
-                    .borrowed_by
-                    .contains_key(&BorrowNode::Reference(*dest))
-                {
-                    instrumented_bytecodes.push(Bytecode::UnpackRef(self.new_attr_id(), *dest));
                 }
             }
             _ => unreachable!(),
