language/move-prover/stackless-bytecode-generator/src/stackless_bytecode_generator.rs
@@ -103,6 +103,7 @@ impl<'a> StacklessBytecodeGenerator<'a> {
             code: self.code,
             local_types: self.local_types,
             return_types: self.func_env.get_return_types(),
+            ref_param_map: BTreeMap::new(),
             acquires_global_resources: self.func_env.get_acquires_global_resources(),
             locations: self.location_table,
             annotations: Annotations::default(),
