language/move-prover/stackless-bytecode-generator/tests/packref/mut_ref.move
@@ -1,0 +1,71 @@
+address 0x1 {
+module TestMutRefs {
+    struct T { value: u64 }
+
+    // Resource to track the sum of values in T
+    resource struct TSum {
+        sum: u64
+    }
+
+    public fun new(x: u64): T acquires TSum {
+        let r = borrow_global_mut<TSum>(0x0);
+        r.sum = r.sum + x;
+        T{value: x}
+    }
+
+    public fun delete(x: T) acquires TSum {
+        let r = borrow_global_mut<TSum>(0x0);
+        let T{value: v} = x;
+        r.sum = r.sum - v;
+    }
+
+    public fun increment(x: &mut T) acquires TSum {
+        x.value = x.value + 1;
+        let r = borrow_global_mut<TSum>(0x0);
+        r.sum = r.sum + 1;
+    }
+
+    public fun increment_invalid(x: &mut T) {
+        x.value = x.value + 1;
+    }
+
+    public fun decrement_invalid(x: &mut T) acquires TSum {
+        x.value = x.value - 1;
+        let r = borrow_global_mut<TSum>(0x0);
+        r.sum = r.sum - 1;
+    }
+
+    fun private_decrement(x: &mut T) acquires TSum {
+        x.value = x.value - 1;
+        let r = borrow_global_mut<TSum>(0x0);
+        r.sum = r.sum - 1;
+    }
+
+    public fun data_invariant(_x: &mut T) {
+    }
+
+    fun private_data_invariant_invalid(_x: &mut T) {
+    }
+
+    fun private_to_public_caller(r: &mut T) acquires TSum {
+        increment(r);
+    }
+
+    fun private_to_public_caller_invalid_data_invariant() acquires TSum {
+        let x = new(1);
+        let r = &mut x;
+        private_decrement(r);
+        increment(r);
+    }
+}
+
+module TestMutRefsUser {
+    use 0x1::TestMutRefs;
+
+    public fun valid() {
+        let x = TestMutRefs::new(4);
+        TestMutRefs::increment(&mut x);
+        TestMutRefs::delete(x);
+    }
+}
+}
