language/move-prover/stackless-bytecode-generator/tests/writeback/libra.move
@@ -1,0 +1,261 @@
+// dep: ../tests/sources/stdlib/modules/transaction.move
+// dep: ../tests/sources/stdlib/modules/vector.move
+
+address 0x0 {
+
+module Libra {
+    use 0x0::Transaction;
+    use 0x0::Vector;
+
+    // A resource representing a fungible token
+    resource struct T<Token> {
+        // The value of the token. May be zero
+        value: u64,
+    }
+
+    // A singleton resource that grants access to `Libra::mint`. Only the Association has one.
+    resource struct MintCapability<Token> { }
+
+    resource struct Info<Token> {
+        // The sum of the values of all Libra::T resources in the system
+        total_value: u128,
+        // Value of funds that are in the process of being burned
+        preburn_value: u64,
+    }
+
+    // A holding area where funds that will subsequently be burned wait while their underyling
+    // assets are sold off-chain.
+    // This resource can only be created by the holder of the MintCapability. An account that
+    // contains this address has the authority to initiate a burn request. A burn request can be
+    // resolved by the holder of the MintCapability by either (1) burning the funds, or (2)
+    // returning the funds to the account that initiated the burn request.
+    // This design supports multiple preburn requests in flight at the same time, including multiple
+    // burn requests from the same account. However, burn requests from the same account must be
+    // resolved in FIFO order.
+    resource struct Preburn<Token> {
+        // Queue of pending burn requests
+        requests: vector<T<Token>>,
+        // Boolean that is true if the holder of the MintCapability has approved this account as a
+        // preburner
+        is_approved: bool,
+    }
+
+    public fun register<Token>() {
+        // Only callable by the Association address
+        Transaction::assert(Transaction::sender() == 0xA550C18, 1);
+        move_to_sender(MintCapability<Token>{ });
+        move_to_sender(Info<Token> { total_value: 0u128, preburn_value: 0 });
+    }
+
+    fun assert_is_registered<Token>() {
+        Transaction::assert(exists<Info<Token>>(0xA550C18), 12);
+    }
+
+    // Return `amount` coins.
+    // Fails if the sender does not have a published MintCapability.
+    public fun mint<Token>(amount: u64): T<Token> acquires Info, MintCapability {
+        mint_with_capability(amount, borrow_global<MintCapability<Token>>(Transaction::sender()))
+    }
+
+    // Burn the coins currently held in the preburn holding area under `preburn_address`.
+    // Fails if the sender does not have a published MintCapability.
+    public fun burn<Token>(
+        preburn_address: address
+    ) acquires Info, MintCapability, Preburn {
+        burn_with_capability(
+            preburn_address,
+            borrow_global<MintCapability<Token>>(Transaction::sender())
+        )
+    }
+
+    // Cancel the oldest burn request from `preburn_address`
+    // Fails if the sender does not have a published MintCapability.
+    public fun cancel_burn<Token>(
+        preburn_address: address
+    ): T<Token> acquires Info, MintCapability, Preburn {
+        cancel_burn_with_capability(
+            preburn_address,
+            borrow_global<MintCapability<Token>>(Transaction::sender())
+        )
+    }
+
+    // Create a new Preburn resource
+    public fun new_preburn<Token>(): Preburn<Token> {
+        assert_is_registered<Token>();
+        Preburn<Token> { requests: Vector::empty(), is_approved: false, }
+    }
+
+    // Mint a new Libra::T worth `value`. The caller must have a reference to a MintCapability.
+    // Only the Association account can acquire such a reference, and it can do so only via
+    // `borrow_sender_mint_capability`
+    public fun mint_with_capability<Token>(
+        value: u64,
+        _capability: &MintCapability<Token>
+    ): T<Token> acquires Info {
+        assert_is_registered<Token>();
+        // TODO: temporary measure for testnet only: limit minting to 1B Libra at a time.
+        // this is to prevent the market cap's total value from hitting u64_max due to excessive
+        // minting. This will not be a problem in the production Libra system because coins will
+        // be backed with real-world assets, and thus minting will be correspondingly rarer.
+        // * 1000000 here because the unit is microlibra
+        Transaction::assert(value <= 1000000000 * 1000000, 11);
+        // update market cap resource to reflect minting
+        let market_cap = borrow_global_mut<Info<Token>>(0xA550C18);
+        market_cap.total_value = market_cap.total_value + (value as u128);
+
+        T<Token> { value }
+    }
+
+    // Send coin to the preburn holding area `preburn_ref`, where it will wait to be burned.
+    public fun preburn<Token>(
+        preburn_ref: &mut Preburn<Token>,
+        coin: T<Token>
+    ) acquires Info {
+        // TODO: bring this back once we can automate approvals in testnet
+        // Transaction::assert(preburn_ref.is_approved, 13);
+        let coin_value = value(&coin);
+        Vector::push_back(
+            &mut preburn_ref.requests,
+            coin
+        );
+        let market_cap = borrow_global_mut<Info<Token>>(0xA550C18);
+        market_cap.preburn_value = market_cap.preburn_value + coin_value
+    }
+
+    // Send coin to the preburn holding area, where it will wait to be burned.
+    // Fails if the sender does not have a published Preburn resource
+    public fun preburn_to_sender<Token>(coin: T<Token>) acquires Info, Preburn {
+        preburn(borrow_global_mut<Preburn<Token>>(Transaction::sender()), coin)
+    }
+
+    // Permanently remove the coins held in the `Preburn` resource stored at `preburn_address` and
+    // update the market cap accordingly. If there are multiple preburn requests in progress, this
+    // will remove the oldest one.
+    // Can only be invoked by the holder of the MintCapability. Fails if the there is no `Preburn`
+    // resource under `preburn_address` or has one with no pending burn requests.
+    public fun burn_with_capability<Token>(
+        preburn_address: address,
+        _capability: &MintCapability<Token>
+    ) acquires Info, Preburn {
+        // destroy the coin at the head of the preburn queue
+        let preburn = borrow_global_mut<Preburn<Token>>(preburn_address);
+        let T { value } = Vector::remove(&mut preburn.requests, 0);
+        // update the market cap
+        let market_cap = borrow_global_mut<Info<Token>>(0xA550C18);
+        market_cap.total_value = market_cap.total_value - (value as u128);
+        market_cap.preburn_value = market_cap.preburn_value - value
+    }
+
+    // Cancel the burn request in the `Preburn` resource stored at `preburn_address` and
+    // return the coins to the caller.
+    // If there are multiple preburn requests in progress, this will cancel the oldest one.
+    // Can only be invoked by the holder of the MintCapability. Fails if the transaction sender
+    // does not have a published Preburn resource or has one with no pending burn requests.
+    public fun cancel_burn_with_capability<Token>(
+        preburn_address: address,
+        _capability: &MintCapability<Token>
+    ): T<Token> acquires Info, Preburn {
+        // destroy the coin at the head of the preburn queue
+        let preburn = borrow_global_mut<Preburn<Token>>(preburn_address);
+        let coin = Vector::remove(&mut preburn.requests, 0);
+        // update the market cap
+        let market_cap = borrow_global_mut<Info<Token>>(0xA550C18);
+        market_cap.preburn_value = market_cap.preburn_value - value(&coin);
+
+        coin
+    }
+
+    // Publish `preburn` under the sender's account
+    public fun publish_preburn<Token>(preburn: Preburn<Token>) {
+        move_to_sender(preburn)
+    }
+
+    // Remove and return the `Preburn` resource under the sender's account
+    public fun remove_preburn<Token>(): Preburn<Token> acquires Preburn {
+        move_from<Preburn<Token>>(Transaction::sender())
+    }
+
+    // Destroys the given preburn resource.
+    // Aborts if `requests` is non-empty
+    public fun destroy_preburn<Token>(preburn: Preburn<Token>) {
+        let Preburn { requests, is_approved: _ } = preburn;
+        Vector::destroy_empty(requests)
+    }
+
+    // Publish `capability` under the sender's account
+    public fun publish_mint_capability<Token>(capability: MintCapability<Token>) {
+        move_to_sender(capability)
+    }
+
+    // Remove and return the MintCapability from the sender's account. Fails if the sender does
+    // not have a published MintCapability
+    public fun remove_mint_capability<Token>(): MintCapability<Token> acquires MintCapability {
+        move_from<MintCapability<Token>>(Transaction::sender())
+    }
+
+    // Return the total value of all Libra in the system
+    public fun market_cap<Token>(): u128 acquires Info {
+        borrow_global<Info<Token>>(0xA550C18).total_value
+    }
+
+    // Return the total value of Libra to be burned
+    public fun preburn_value<Token>(): u64 acquires Info {
+        borrow_global<Info<Token>>(0xA550C18).preburn_value
+    }
+
+    // Create a new Libra::T with a value of 0
+    public fun zero<Token>(): T<Token> {
+        // prevent silly coin types (e.g., Libra<bool>) from being created
+        assert_is_registered<Token>();
+        T { value: 0 }
+    }
+
+    // Public accessor for the value of a coin
+    public fun value<Token>(coin_ref: &T<Token>): u64 {
+        coin_ref.value
+    }
+
+    // Splits the given coin into two and returns them both
+    // It leverages `withdraw` for any verifications of the values
+    public fun split<Token>(coin: T<Token>, amount: u64): (T<Token>, T<Token>) {
+        let other = withdraw(&mut coin, amount);
+        (coin, other)
+    }
+
+    // "Divides" the given coin into two, where original coin is modified in place
+    // The original coin will have value = original value - `value`
+    // The new coin will have a value = `value`
+    // Fails if the coins value is less than `value`
+    public fun withdraw<Token>(coin_ref: &mut T<Token>, value: u64): T<Token> {
+        // Check that `amount` is less than the coin's value
+        Transaction::assert(coin_ref.value >= value, 10);
+
+        // Split the coin
+        coin_ref.value = coin_ref.value - value;
+        T { value }
+    }
+
+    // Merges two coins and returns a new coin whose value is equal to the sum of the two inputs
+    public fun join<Token>(coin1: T<Token>, coin2: T<Token>): T<Token>  {
+        deposit(&mut coin1, coin2);
+        coin1
+    }
+
+    // "Merges" the two coins
+    // The coin passed in by reference will have a value equal to the sum of the two coins
+    // The `check` coin is consumed in the process
+    public fun deposit<Token>(coin_ref: &mut T<Token>, check: T<Token>) {
+        let T { value } = check;
+        coin_ref.value= coin_ref.value + value;
+    }
+
+    // Destroy a coin
+    // Fails if the value is non-zero
+    // The amount of Libra::T in the system is a tightly controlled property,
+    // so you cannot "burn" any non-zero amount of Libra::T
+    public fun destroy_zero<Token>(coin: T<Token>) {
+        let T<Token> { value } = coin;
+        Transaction::assert(value == 0, 11);
+    }
+}
+}
